

## CONVEX OPTIMIZATION HW

SPRING 2025

1. LASSO Problem numerical optimization

**Solution.** See jupyter notebook file.

2. Write as a linear program.

(a)  $\min \|A\mathbf{x} - \mathbf{b}\|_1.$

**Solution.** The 1-norm can be expressed as

$$\|A\mathbf{x} - \mathbf{b}\|_1 = \sum_{i=1}^m |(A\mathbf{x} - \mathbf{b})_i|.$$

To handle the absolute values, we introduce nonnegative auxiliary variables  $t_i$  for  $i = 1, 2, \dots, m$ , and require

$$t_i \geq (A\mathbf{x} - \mathbf{b})_i \quad \text{and} \quad t_i \geq -(A\mathbf{x} - \mathbf{b})_i,$$

with  $t_i \geq 0$ . This allows us to reformulate the original problem as

$$\min_{\mathbf{x}, t} \sum_{i=1}^m t_i,$$

subject to

$$\begin{aligned} A\mathbf{x} - \mathbf{b} &\leq t, \\ -A\mathbf{x} + \mathbf{b} &\leq t, \\ t &\geq 0, \end{aligned}$$

where  $t$  denotes the vector with components  $t_i$ .

(b)  $\min \|\mathbf{x}\|_1$  s.t.  $\|A\mathbf{x} - \mathbf{b}\|_\infty \leq 1.$

**Solution.** Again, note that the 1-norm of  $\mathbf{x}$  is given by

$$\|\mathbf{x}\|_1 = \sum_{j=1}^n |x_j|.$$

To handle the absolute values, we introduce nonnegative auxiliary variables  $u_j \geq 0$  for  $j = 1, 2, \dots, n$ , and impose

$$u_j \geq x_j \quad \text{and} \quad u_j \geq -x_j.$$

Next, the constraint  $\|A\mathbf{x} - \mathbf{b}\|_\infty \leq 1$  means that the maximum absolute value among the entries of  $A\mathbf{x} - \mathbf{b}$  is at most 1. In other words, for each row  $i$ , we have

$$|(A\mathbf{x} - \mathbf{b})_i| \leq 1.$$

This can be split into the two linear inequalities

$$A\mathbf{x} - \mathbf{b} \leq \mathbf{1}, \quad \text{and} \quad -A\mathbf{x} + \mathbf{b} \leq \mathbf{1},$$

where  $\mathbf{1}$  is the vector of ones. Thus, the final linear programming formulation is given by

$$\begin{aligned} \min_{\mathbf{u}, \mathbf{x}} \quad & \sum_{j=1}^n u_j \\ \text{subject to} \quad & u_j \geq x_j, \quad j = 1, \dots, n, \\ & u_j \geq -x_j, \quad j = 1, \dots, n, \\ & A\mathbf{x} - \mathbf{b} \leq \mathbf{1}, \\ & -A\mathbf{x} + \mathbf{b} \leq \mathbf{1}, \\ & u_j \geq 0, \quad j = 1, \dots, n. \end{aligned}$$

### 3. Lagrange Duality

**Solution. Feasible Set:** The inequality

$$(x - 2)(x - 4) \leq 0$$

has roots at  $x = 2$  and  $x = 4$ , and it holds for

$$x \in [2, 4].$$

**Optimal Solution:** Since  $f(x) = x^2 + 1$  is strictly convex, and its stationary point is not in the feasibility set, so its minimum in the feasible set is attained at one of the boundary points. Evaluating,

$$f(2) = 2^2 + 1 = 5, \quad f(4) = 4^2 + 1 = 17.$$

Thus, the optimal solution is  $x = 2$  with the optimal value  $f(2) = 5$ . Introduce the Lagrange multiplier  $\lambda \geq 0$  for the constraint. The Lagrangian is

$$\begin{aligned} L(x, \lambda) &= x^2 + 1 + \lambda(x - 2)(x - 4) \\ &= x^2 + 1 + \lambda(x^2 - 6x + 8) \\ &= (1 + \lambda)x^2 - 6\lambda x + (1 + 8\lambda). \end{aligned}$$

The dual function is defined as

$$g(\lambda) = \inf_{x \in \mathbb{R}} L(x, \lambda).$$

Since  $L(x, \lambda)$  is quadratic in  $x$  with  $1 + \lambda > 0$  (for  $\lambda \geq 0$ ), its minimum occurs at

$$\frac{\partial L}{\partial x} = 2(1 + \lambda)x - 6\lambda = 0 \implies x^* = \frac{3\lambda}{1 + \lambda}.$$

Substitute  $x^*$  into  $L(x, \lambda)$ :

$$\begin{aligned} g(\lambda) &= L\left(\frac{3\lambda}{1 + \lambda}, \lambda\right) \\ &= (1 + \lambda) \left(\frac{3\lambda}{1 + \lambda}\right)^2 - 6\lambda \left(\frac{3\lambda}{1 + \lambda}\right) + (1 + 8\lambda) \\ &= \frac{9\lambda^2}{1 + \lambda} - \frac{18\lambda^2}{1 + \lambda} + (1 + 8\lambda) \\ &= 1 + 8\lambda - \frac{9\lambda^2}{1 + \lambda} = \frac{1 + 9\lambda - \lambda^2}{1 + \lambda}, \quad \lambda \geq 0. \end{aligned}$$

**Dual Problem:** The dual problem is

$$\max_{\lambda \geq 0} g(\lambda).$$

The dual function  $g(\lambda)$  is the pointwise infimum of a family of functions affine in  $\lambda$ . Therefore,  $g$ . To maximize  $g(\lambda)$  for  $\lambda \geq 0$ , we differentiate using the quotient rule. Define

$$N(\lambda) = 1 + 9\lambda - \lambda^2, \quad D(\lambda) = 1 + \lambda.$$

Then

$$g'(\lambda) = \frac{N'(\lambda)D(\lambda) - N(\lambda)D'(\lambda)}{(D(\lambda))^2},$$

with

$$N'(\lambda) = 9 - 2\lambda \quad \text{and} \quad D'(\lambda) = 1.$$

Thus,

$$\begin{aligned} g'(\lambda) &= \frac{(9 - 2\lambda)(1 + \lambda) - (1 + 9\lambda - \lambda^2)}{(1 + \lambda)^2} \\ &= \frac{[9 + 7\lambda - 2\lambda^2] - (1 + 9\lambda - \lambda^2)}{(1 + \lambda)^2} \\ &= \frac{8 - 2\lambda - \lambda^2}{(1 + \lambda)^2}. \end{aligned}$$

Setting the numerator equal to zero,

$$8 - 2\lambda - \lambda^2 = 0 \implies \lambda^2 + 2\lambda - 8 = 0.$$

The solutions are

$$\lambda = \frac{-2 \pm \sqrt{4 + 32}}{2} = \frac{-2 \pm 6}{2},$$

giving  $\lambda = 2$  and  $\lambda = -4$ . Since  $\lambda \geq 0$  we take  $\lambda^* = 2$ . Evaluating the dual function at  $\lambda = 2$ ,

$$g(2) = \frac{1 + 9 \cdot 2 - 2^2}{1 + 2} = \frac{1 + 18 - 4}{3} = \frac{15}{3} = 5.$$

**Strong Duality:** The optimal value of the primal problem is  $f(2) = 2^2 + 1 = 5$ . Since the dual optimal value is also 5, strong duality holds.

*For the plots, see the jupyter notebook file.*

#### 4. Duality of Boolean LP

##### (a) Lagrange Duality

**Solution.** The Lagrangian is

$$\begin{aligned} L(x, \mu, \nu) &= c^\top x + \mu^\top (Ax - b) - \nu^\top x + x^\top \text{diag}(\nu)x \\ &= x^\top \text{diag}(\nu)x + (c + A^\top \mu - \nu)^\top x - b^\top \mu. \end{aligned}$$

Setting  $\nabla_x f = 0$  gives

$$2 \text{diag}(\nu)x^* + (c + A^\top \mu - \nu) = 0 \implies x^* = -\frac{1}{2} \text{diag}(\nu)^{-1} (c + A^\top \mu - \nu).$$

Substituting back:

$$\begin{aligned} x^{*\top} \text{diag}(\nu)x^* &= \frac{1}{4} (c + A^\top \mu - \nu)^\top \text{diag}(\nu)^{-1} (c + A^\top \mu - \nu), \\ (c + A^\top \mu - \nu)^\top x^* &= -\frac{1}{2} (c + A^\top \mu - \nu)^\top \text{diag}(\nu)^{-1} (c + A^\top \mu - \nu), \end{aligned}$$

so their sum is

$$x^{*\top} \text{diag}(\nu)x^* + (c + A^\top \mu - \nu)^\top x^* = -\frac{1}{4} (c + A^\top \mu - \nu)^\top \text{diag}(\nu)^{-1} (c + A^\top \mu - \nu).$$

Hence the dual function is

$$g(\mu, \nu) = \inf_x L(x, \mu, \nu) = -b^\top \mu - \frac{1}{4}(c + A^\top \mu - \nu)^\top \text{diag}(\nu)^{-1}(c + A^\top \mu - \nu),$$

or, in component form,

$$g(\mu, \nu) = -b^\top \mu - \frac{1}{4} \sum_{i=1}^n \frac{(c_i + a_i^\top \mu - \nu_i)^2}{\nu_i}, \quad \nu \succeq 0.$$

Thus minimizing over  $x$  gives the dual function

$$g(\mu, \nu) = \begin{cases} -b^\top \mu - (1/4) \sum_{i=1}^n (c_i + a_i^\top \mu - \nu_i)^2 / \nu_i & \nu \succeq 0 \\ -\infty & \text{otherwise} \end{cases}$$

where  $a_i$  is the  $i$ th column of  $A$ . The resulting dual problem is

$$\begin{aligned} & \text{maximize} && -b^\top \mu - \frac{1}{4} \sum_{i=1}^n \frac{(c_i + a_i^\top \mu - \nu_i)^2}{\nu_i} \\ & \text{subject to} && \nu \succeq 0, \quad \mu \succeq 0. \end{aligned}$$

For each  $i$ , define

$$h_i(\nu_i) = -\frac{(c_i + a_i^\top \mu - \nu_i)^2}{\nu_i}, \quad \nu_i \geq 0.$$

We maximize  $h_i$  by setting

$$0 = \frac{d}{d\nu_i} \left[ -\frac{(c_i + a_i^\top \mu - \nu_i)^2}{\nu_i} \right] = \frac{(c_i + a_i^\top \mu)^2}{\nu_i^2} - 1 \implies \nu_i^* = |c_i + a_i^\top \mu|.$$

Substituting back,

$$\sup_{\nu_i \geq 0} h_i(\nu_i) = \begin{cases} 4(c_i + a_i^\top \mu), & c_i + a_i^\top \mu \leq 0, \\ 0, & c_i + a_i^\top \mu \geq 0, \end{cases} = \min\{0, 4(c_i + a_i^\top \mu)\}.$$

Therefore the  $\nu$ -optimized dual becomes

$$\begin{aligned} \sup_{\nu \succeq 0} g(\mu, \nu) &= -b^\top \mu - \frac{1}{4} \sum_{i=1}^n \sup_{\nu_i \geq 0} \left[ -\frac{(c_i + a_i^\top \mu - \nu_i)^2}{\nu_i} \right] \\ &= -b^\top \mu + \sum_{i=1}^n \min\{0, c_i + a_i^\top \mu\}. \end{aligned}$$

So the final dual problem is

$$\begin{aligned} & \max_{\mu} && -b^\top \mu + \sum_{i=1}^n \min\{0, c_i + a_i^\top \mu\}, \\ & \text{s.t.} && \mu \succeq 0. \end{aligned}$$

(b) LP relaxation

**Solution.** The Lagrangian function of the LP relaxation is

$$\begin{aligned} L(x, u, v, w) &= c^\top x + u^\top (Ax - b) - v^\top x + w^\top (x - 1) \\ &= (c + A^\top u - v + w)^\top x - b^\top u - \mathbf{1}^\top w, \end{aligned}$$

where  $v$  and  $w$  are Lagrange multipliers. Then minizing over  $x$  by first order condition gives the dual objective function

$$g(u, v, w) = \begin{cases} -b^\top u - \mathbf{1}^\top w & A^\top u - v + w + c = 0 \\ -\infty & \text{otherwise} \end{cases}$$

The dual problem is therefore

$$\begin{aligned} & \text{maximize} && -b^\top u - \mathbf{1}^\top w \\ & \text{subject to} && A^\top u - v + w + c = 0 \\ & && u \succeq 0, v \succeq 0, w \succeq 0, \end{aligned}$$

which is equivalent to the Lagrange relaxation problem derived above by marginally optimizing  $v$  and  $w$  first.

5. Calculate subgradient

(a)  $f(\mathbf{x}) = \max_i |\mathbf{a}_i^\top \mathbf{x} + b_i|$

**Solution.** Let

$$r_i = \mathbf{a}_i^\top \mathbf{x} + b_i, \quad i = 1, \dots, m,$$

and let

$$f(\mathbf{x}) = \max_i |r_i| = \alpha.$$

Define the active set  $I \subseteq \{1, \dots, m\}$  by

$$I = \{i \mid |r_i| = \alpha\}.$$

For each  $i$  in the active set  $I$ , the subgradient for the term  $|\mathbf{a}_i^\top \mathbf{x} + b_i|$  can be written as

$$\mathbf{g}_i = \text{sign}(r_i) \mathbf{a}_i = \begin{cases} +\mathbf{a}_i, & r_i > 0, \\ -\mathbf{a}_i, & r_i < 0, \\ \text{any vector in } [-1, +1]\mathbf{a}_i, & r_i = 0. \end{cases}$$

Because  $f(\mathbf{x})$  is the maximum of these absolute-value terms, any subgradient  $\mathbf{g}$  of  $f$  at  $\mathbf{x}$  must lie in the *convex hull* of the  $\mathbf{g}_i$ 's coming from the active indices:

$$\mathbf{g} \in \text{conv} \left\{ \text{sign}(r_i) \mathbf{a}_i : i \in I \right\}.$$

In other words, pick any convex combination of the vectors  $\text{sign}(r_i) \mathbf{a}_i$  for  $i$  in  $I$ .

(b)  $f(\mathbf{x}) = \mathbf{x}_{[1]} + \dots + \mathbf{x}_{[k]}$ , where  $\mathbf{x}_{[1]} \geq \mathbf{x}_{[2]} \geq \dots \geq \mathbf{x}_{[n]}$  denote the components of  $\mathbf{x}$  in descending order.

**Solution.** Let  $S$  be the set of indices corresponding to the  $k$  largest entries of  $\mathbf{x}$ . That is,

$$S = \{i : x_i \text{ is among the top } k \text{ values of } \mathbf{x}\}.$$

Suppose  $\mathbf{x}_{[k]} > \mathbf{x}_{[k+1]}$ . Then  $S$  has exactly  $k$  distinct elements, and a subgradient is the vector

$$\mathbf{g} \quad \text{where} \quad g_i = \begin{cases} 1, & i \in S, \\ 0, & i \notin S. \end{cases}$$

If there is a tie for the  $k$ -th largest value (i.e.,  $\mathbf{x}_{[k]} = \mathbf{x}_{[k+1]}$ ), we let:

$$\ell = \#\{i : x_i > \mathbf{x}_{[k]}\}, \quad T = \{i : x_i = \mathbf{x}_{[k]}\}.$$

Then we must assign  $g_i = 1$  to indices strictly greater than  $\mathbf{x}_{[k]}$ , and  $g_i = 0$  for indices strictly less. For  $i$  in  $T$ , assign  $g_i$  in  $[0, 1]$  so that

$$\sum_{i \in T} g_i = k - \ell.$$

Hence the subgradient belongs to the convex set of all such assignments.

(c)  $f(\mathbf{x}) = \inf_{\mathbf{A}\mathbf{y} \leq \mathbf{b}} \|\mathbf{x} - \mathbf{y}\|_2^2$ .

**Solution.** This is the squared distance from  $\mathbf{x}$  to the polyhedron  $C = \{\mathbf{y} : A\mathbf{y} \preceq \mathbf{b}\}$ . Let

$$f(\mathbf{x}) = \|\mathbf{x} - \Pi_C(\mathbf{x})\|_2^2$$

where  $\Pi_C(\mathbf{x})$  denotes the Euclidean projection of  $\mathbf{x}$  onto  $C$ :

$$\Pi_C(\mathbf{x}) = \arg \min_{\mathbf{y} \in C} \|\mathbf{x} - \mathbf{y}\|_2^2.$$

If  $\mathbf{x} \in C$ . Then  $f(\mathbf{x}) = 0$  and  $\mathbf{x}$  itself is a closest point in  $C$ . In a neighborhood inside  $C$ ,  $f$  stays 0, so the subgradient at  $\mathbf{x}$  is  $\mathbf{0}$ . If  $\mathbf{x} \notin C$ . Let  $\mathbf{y}^* \in \Pi_C(\mathbf{x})$ . Then

$$f(\mathbf{x}) = \|\mathbf{x} - \mathbf{y}^*\|_2^2.$$

The gradient (w.r.t.  $\mathbf{x}$ ) of  $\|\mathbf{x} - \mathbf{y}^*\|_2^2$  is

$$\nabla_{\mathbf{x}} \|\mathbf{x} - \mathbf{y}^*\|_2^2 = 2(\mathbf{x} - \mathbf{y}^*).$$

Thus a subgradient of  $f$  at  $\mathbf{x}$  is

$$\mathbf{g} = 2(\mathbf{x} - \mathbf{y}^*),$$

for the  $\mathbf{y}^*$  that is the projection  $\Pi_C(\mathbf{x})$ .

(d)  $f(\mathbf{x}) = \sup_{A\mathbf{y} \preceq \mathbf{b}} \mathbf{y}^\top \mathbf{x}.$

**Solution.** Since  $f(\mathbf{x}) = \sup_{\mathbf{y} \in P} \mathbf{y}^\top \mathbf{x}$  is just the support function of  $P := \{A\mathbf{y} \preceq \mathbf{b}\}$ , we immediately conclude:

$$\partial f(\mathbf{x}) = \text{conv}(\{\mathbf{y}^* \in P : \mathbf{y}^{*\top} \mathbf{x} = f(\mathbf{x})\}).$$

Let  $\mathbf{y}^*$  be any optimal solution of  $\max_{\mathbf{y} \in P} \mathbf{y}^\top \mathbf{x}$ . If there is a unique solution, the subgradient is just  $\{\mathbf{y}^*\}$ .

## 6. Subgradient of $\|x\|_2$ .

**Solution.** When  $x \neq 0$ ,  $f$  is differentiable at  $x$ . Recall that for  $x \neq 0$ , the gradient is

$$\nabla f(x) = \frac{x}{\|x\|_2}.$$

For a convex function that is differentiable at  $x \neq 0$ , the subdifferential coincides with the set containing its gradient. Hence,

$$\partial f(x) = \left\{ \frac{x}{\|x\|_2} \right\}.$$

When  $x = 0$ , the function  $f$  is not differentiable. We use the definition of a subgradient for a convex function:  $g$  is in the subdifferential  $\partial f(0)$  if and only if

$$f(y) \geq f(0) + \langle g, y - 0 \rangle \quad \text{for all } y.$$

Since  $f(0) = 0$ , we need

$$\|y\|_2 \geq \langle g, y \rangle \quad \text{for all } y.$$

By Cauchy-Schwarz inequality, for all  $g$  such that  $\|g\|_2 \leq 1$  we obtain

$$\|y\|_2 \geq \|y\|_2 \|g\|_2 \geq \langle g, y \rangle,$$

we therefore have

$$\partial f(0) = \{g : \|g\|_2 \leq 1\}.$$

## 7. Compute proximal operators.

(a)  $f(x) = \frac{1}{2}x^\top Ax + b^\top x + c, \quad \text{where } A \in S_n^+.$

**Solution.** We wish to compute the proximal operator defined by

$$\text{prox}_f(v) = \arg \min_{x \in \mathbb{R}^n} \left\{ f(x) + \frac{1}{2} \|x - v\|_2^2 \right\}.$$

We wish to solve

$$\min_{x \in \mathbb{R}^n} \left\{ \frac{1}{2} x^\top A x + b^\top x + c + \frac{1}{2} \|x - v\|_2^2 \right\}.$$

Define

$$\varphi(x) = \frac{1}{2} x^\top A x + b^\top x + \frac{1}{2} \|x - v\|_2^2.$$

Taking the gradient with respect to  $x$ , we have

$$\nabla \varphi(x) = Ax + b + (x - v).$$

Setting the gradient equal to zero gives:

$$Ax + b + x - v = 0.$$

Solving for the optimal solution

$$\text{prox}_f(v) = x = (A + I)^{-1}(v - b).$$

(b)  $f(x) = -\sum_{i=1}^n \log x_i$  where  $x \in \mathbb{R}_+^n$ .

**Solution.** We want to compute

$$\text{prox}_f(v) = \arg \min_{x \in \mathbb{R}_+^n} \left\{ -\sum_{i=1}^n \log x_i + \frac{1}{2} \|x - v\|_2^2 \right\}.$$

Since the objective is separable, we solve the scalar subproblem for each  $i$ :

$$x'_i = \arg \min_{x_i > 0} \left\{ -\log x_i + \frac{1}{2} (x_i - v_i)^2 \right\}.$$

Taking the derivative with respect to  $x_i$  and setting it to zero:

$$-\frac{1}{x_i} + (x_i - v_i) = 0 \implies x_i^2 - v_i x_i - 1 = 0.$$

Solving the quadratic equation for  $x_i$  yields

$$x_i = \frac{v_i \pm \sqrt{v_i^2 + 4}}{2}.$$

Since  $x_i > 0$ , we take

$$x'_i = \frac{v_i + \sqrt{v_i^2 + 4}}{2}.$$

Hence, the proximal operator of  $f$  evaluated at  $v$  is given coordinate-wise by

$$(\text{prox}_f(v))_i = \frac{v_i + \sqrt{v_i^2 + 4}}{2}, \quad i = 1, \dots, n.$$

(c)  $f(x) = \|x\|_2$ .

**Solution.** We wish to solve

$$\text{prox}_f(v) = \arg \min_{x \in \mathbb{R}^n} \left\{ \|x\|_2 + \frac{1}{2} \|x - v\|_2^2 \right\}.$$

A key observation is that, because the Euclidean norm  $\|\cdot\|_2$  is rotationally symmetric, the minimizer  $x$  must lie on the same ray as  $v$ . Thus we can write

$$x = tv \quad \text{for some scalar } t \geq 0.$$

Substituting  $x = tv$  into the objective function yields

$$\|x\|_2 = t\|v\|_2, \quad \|x - v\|_2^2 = \|(t - 1)v\|_2^2 = (t - 1)^2\|v\|_2^2.$$

Hence the optimization problem reduces to

$$\min_{t \geq 0} \left\{ t\|v\|_2 + \frac{1}{2}(t - 1)^2\|v\|_2^2 \right\}.$$

Let us define

$$\phi(t) = t\|v\|_2 + \frac{1}{2}(t - 1)^2\|v\|_2^2.$$

Taking the derivative with respect to  $t$ :

$$\frac{d\phi}{dt} = \|v\|_2 + (t - 1)\|v\|_2^2.$$

Setting this derivative to zero for an unconstrained minimizer:

$$\|v\|_2 + (t - 1)\|v\|_2^2 = 0 \implies t = 1 - \frac{1}{\|v\|_2}.$$

Because  $t \geq 0$ , we require

$$1 - \frac{1}{\|v\|_2} \geq 0 \implies \|v\|_2 \geq 1.$$

Thus,

$$t = \begin{cases} 1 - \frac{1}{\|v\|_2}, & \text{if } \|v\|_2 \geq 1, \\ 0, & \text{if } \|v\|_2 < 1. \end{cases}$$

Then the result can be written as

$$\text{prox}_{\|\cdot\|_2}(v) = \left(1 - \frac{1}{\|v\|_2}\right)_+ v.$$

(d)  $f(x) = \|x\|_0$ , where  $\|x\|_0 = \text{card}\{x_i : x_i \neq 0, i = 1, \dots, n\}$ .

**Solution.** We want

$$\text{prox}_f(v) = \arg \min_{x \in \mathbb{R}^n} \left\{ \|x\|_0 + \frac{1}{2}\|x - v\|_2^2 \right\},$$

with  $\|x\|_0 = \text{card}\{i : x_i \neq 0\}$ . Because the objective is separable, consider the scalar problem for each coordinate  $i$ :

$$\min_{x_i \in \mathbb{R}} \left\{ \mathbf{1}_{\{x_i \neq 0\}} + \frac{1}{2}(x_i - v_i)^2 \right\}.$$

Here  $\mathbf{1}_{\{x_i \neq 0\}} = 0$  if  $x_i = 0$ , and 1 otherwise. Thus if  $x_i = 0$ , the cost is  $\frac{1}{2}v_i^2$ . If  $x_i \neq 0$ , the optimal choice is  $x_i = v_i$  and the cost is 1. Hence we compare  $\frac{1}{2}v_i^2$  with 1. If  $\frac{1}{2}v_i^2 \leq 1$ , it is cheaper to set  $x_i = 0$ . Otherwise, choose  $x_i = v_i$ . That is,

$$(\text{prox}_f(v))_i = \begin{cases} 0, & |v_i| \leq \sqrt{2}, \\ v_i, & |v_i| > \sqrt{2}. \end{cases}$$

## 8. Proximal Operator of The Group Lasso Problem

**Solution.** We take the definition

$$\text{prox}_{h,t}(x) = \arg \min_{z \in \mathbb{R}^p} \left\{ \frac{1}{2t}\|x - z\|_2^2 + h(z) \right\},$$

where

$$h(z) = \lambda \sum_{j=1}^J \omega_j \|z_{(j)}\|_2,$$



and  $z_{(j)}$  is the  $j$ th block of  $z$ . Since  $h$  is separable over the blocks, the minimization decouples:

$$[\text{prox}_{h,t}(x)]_{(j)} = \arg \min_{z_{(j)} \in \mathbb{R}^{d_j}} \frac{1}{2t} \|x_{(j)} - z_{(j)}\|_2^2 + \lambda \omega_j \|z_{(j)}\|_2.$$

Define

$$\alpha_j = t\lambda\omega_j,$$

and note that multiplying the objective by the positive constant  $t$  does not change the minimizer. Equivalently we solve

$$z^* = \arg \min_{z \in \mathbb{R}^{d_j}} \underbrace{\frac{1}{2} \|z - x\|_2^2 + \alpha_j \|z\|_2}_{\Phi(z)}, \quad x = x_{(j)}.$$

(i) If  $x = 0$ , clearly  $z^* = 0$ .

(ii) Otherwise write

$$u = \frac{x}{\|x\|_2}, \quad \|u\|_2 = 1, \quad z = ru + w, \quad u^\top w = 0.$$

Then

$$\|z - x\|_2^2 = (r - \|x\|_2)^2 + \|w\|_2^2, \quad \|z\|_2 \geq |r|.$$

It is suboptimal to have  $\|w\|_2 > 0$ , so at the optimum  $w = 0$  and  $z = ru$ ,  $r \geq 0$ .

(iii) Substituting  $z = ru$  gives

$$\Phi(r) = \frac{1}{2}(r - \|x\|_2)^2 + \alpha_j r = \frac{1}{2}r^2 - r\|x\|_2 + \alpha_j r + \text{const.}$$

Differentiate w.r.t.  $r$ :

$$\frac{d\Phi}{dr} = r - \|x\|_2 + \alpha_j \implies r = \|x\|_2 - \alpha_j \quad (\text{stationary}).$$

Enforcing  $r \geq 0$  yields

$$r^* = \max\{0, \|x\|_2 - \alpha_j\}.$$

(iv) Hence

$$z^* = r^* u = \begin{cases} (\|x\|_2 - \alpha_j) \frac{x}{\|x\|_2}, & \|x\|_2 > \alpha_j, \\ 0, & \|x\|_2 \leq \alpha_j. \end{cases}$$

Equivalently,

$$z^* = \max\left\{0, 1 - \frac{\alpha_j}{\|x\|_2}\right\} x = \max\left\{0, 1 - \frac{t\lambda\omega_j}{\|x\|_2}\right\} x.$$

Putting everything together, we have

$$[\text{prox}_{h,t}(x)]_{(j)} = \left(1 - \frac{t\lambda\omega_j}{\|x_{(j)}\|_2}\right)^+ x_{(j)}, \quad j = 1, 2, \dots, J.$$

*Algorithms see Jupyter Notebook file.*